src/Experiments/NewPipeline/Rewriter.v
@@ -1904,7 +1904,7 @@ Module Compilers.
             ; make_rewrite_step (* _step, so that if one of the arguments is concrete, we automatically get the rewrite rule for [Z_cast] applying to it *)
                 (#pattern.ident.Z_cast2 @ (??, ??)) (fun r x y => (#(ident.Z_cast (fst r)) @ $x, #(ident.Z_cast (snd r)) @ $y))
 
-            ; make_rewriteol (-??) (fun e => (llet v := e in -$v)  when  negb (SubstVarLike.is_var_fst_snd_pair_opp e)) (* inline negation when the rewriter wouldn't already inline it *)
+            ; make_rewriteol (-??) (fun e => (llet v := e in -$v)  when  negb (SubstVarLike.is_var_fst_snd_pair_opp_cast e)) (* inline negation when the rewriter wouldn't already inline it *)
            ].
 
       Definition arith_with_casts_rewrite_rules : rewrite_rulesT
@@ -2200,7 +2200,7 @@ Z.mul @@ (?x >> 128, ?y >> 128)             --> mulhh @@ (x, y)
                     Compile.option_bind' pident_unify_unknown invert_bind_args_unknown Compile.normalize_deep_rewrite_rule
                     Compile.reflect UnderLets.reify_and_let_binds_base_cps Compile.reify Compile.reify_and_let_binds_cps
                     Compile.value'
-                    SubstVarLike.is_var_fst_snd_pair_opp
+                    SubstVarLike.is_var_fst_snd_pair_opp_cast
                  ] in rewrite_head0).
     Ltac timed_make_rewrite_head1 rewrite_head0 pr2_rewrite_rules :=
       constr:(ltac:(time (idtac; let v := make_rewrite_head1 rewrite_head0 pr2_rewrite_rules in exact v))).
